flowstlc/Flowstlc.lean
@@ -1,1 +1,11 @@
 import Flowstlc.Basics
+import Flowstlc.CallByValue
+import Flowstlc.Confluence
+import Flowstlc.Context
+import Flowstlc.Decidable
+import Flowstlc.MultiSubst
+import Flowstlc.Normalization
+import Flowstlc.OpenClose
+import Flowstlc.Reductions
+import Flowstlc.SecurityLevel
+import Flowstlc.Typing
